Deploying to gh-pages from @ xubaiw/reservoir-index@2f87a4a531528c3b3eaba917bfed674c50acc477 🚀

git/cruhland/lean4-axiomatic/Lean4Axiomatic/Natural/Addition.lean
@@ -1,9 +1,13 @@
 import Lean4Axiomatic.Natural.Core
 
+/-!
+# Natural number addition
+-/
+
 namespace Lean4Axiomatic.Natural
 
 /-!
-# Definition and properties of natural number addition
+## Axioms
 -/
 
 /--
@@ -11,7 +15,7 @@ Definition of addition, and properties that it must satisfy.
 
 All other properties of addition can be derived from these.
 -/
-class Addition.Base (ℕ : Type) [Core ℕ] where
+class Addition (ℕ : Type) [Core ℕ] :=
   /-- Definition of and syntax for addition. -/
   addOp : Add ℕ
 
@@ -21,61 +25,228 @@ class Addition.Base (ℕ : Type) [Core ℕ] where
   /-- Incrementing the left term in a sum increments the result. -/
   step_add {n m : ℕ} : step n + m ≃ step (n + m)
 
-attribute [instance] Addition.Base.addOp
+attribute [instance] Addition.addOp
 
-/-- Properties that follow from those provided in `Addition.Base`. -/
-class Addition.Derived (ℕ : Type) [Core ℕ] extends Addition.Base ℕ where
-  /-- Adding zero to any natural number (on the right) leaves it unchanged. -/
-  add_zero {n : ℕ} : n + 0 ≃ n
+export Addition (addOp step_add zero_add)
 
-  /-- Adding zero to a natural number produces the same natural number. -/
-  add_identity : AA.Identity (α := ℕ) 0 (· + ·)
+/-!
+## Derived properties
+-/
 
-  /-- Incrementing the right term in a sum increments the result. -/
-  add_step {n m : ℕ} : n + step m ≃ step (n + m)
+variable {ℕ : Type}
+variable [Core ℕ]
+variable [Axioms ℕ]
+variable [Addition ℕ]
 
-  /-- Incrementing a sum is equivalent to incrementing one of its terms. -/
-  add_semicompatible_step : AA.Semicompatible (α := ℕ) step (· + ·)
+/-- Adding zero to any natural number (on the right) leaves it unchanged. -/
+theorem add_zero {n : ℕ} : n + 0 ≃ n := by
+  apply ind_on (motive := λ n => n + 0 ≃ n) n
+  case zero =>
+    show 0 + 0 ≃ 0
+    calc
+      0 + (0 : ℕ) ≃ _ := Addition.zero_add
+      0           ≃ _ := Rel.refl
+  case step =>
+    intro n (ih : n + 0 ≃ n)
+    show step n + 0 ≃ step n
+    calc
+      step n + 0   ≃ _ := Addition.step_add
+      step (n + 0) ≃ _ := AA.subst₁ ih
+      step n       ≃ _ := Rel.refl
 
-  /--
-  Addition preserves equality of natural numbers; two equal natural numbers are
-  still equal after the same quantity is added to both (on the left or right).
-  -/
-  add_substitutive : AA.Substitutive₂ (α := ℕ) (· + ·) AA.tc (· ≃ ·) (· ≃ ·)
+instance add_identity : AA.Identity (α := ℕ) 0 (· + ·) := {
+  identityL := AA.IdentityOn.mk Addition.zero_add
+  identityR := AA.IdentityOn.mk add_zero
+}
 
-  /-- Adding one is the same as incrementing. -/
-  add_one_step {n : ℕ} : n + 1 ≃ step n
+/-- Incrementing the right term in a sum increments the result. -/
+theorem add_step {n m : ℕ} : n + step m ≃ step (n + m) := by
+  apply ind_on (motive := λ n => n + step m ≃ step (n + m)) n
+  case zero =>
+    show 0 + step m ≃ step (0 + m)
+    calc
+      0 + step m   ≃ _ := Addition.zero_add
+      step m       ≃ _ := AA.subst₁ (Rel.symm Addition.zero_add)
+      step (0 + m) ≃ _ := Rel.refl
+  case step =>
+    intro n (ih : n + step m ≃ step (n + m))
+    show step n + step m ≃ step (step n + m)
+    calc
+      step n + step m     ≃ _ := Addition.step_add
+      step (n + step m)   ≃ _ := AA.subst₁ ih
+      step (step (n + m)) ≃ _ := AA.subst₁ (Rel.symm Addition.step_add)
+      step (step n + m)   ≃ _ := Rel.refl
 
-  /-- Exchanging the operands of an addition does not change the result. -/
-  add_commutative : AA.Commutative (α := ℕ) (· + ·)
+instance add_semicompatible_step : AA.Semicompatible (α := ℕ) step (· + ·) := {
+  semicompatibleL := AA.SemicompatibleOn.mk (Rel.symm Addition.step_add)
+  semicompatibleR := AA.SemicompatibleOn.mk (Rel.symm add_step)
+}
 
-  /-- The grouping of the terms in a sum doesn't matter. -/
-  add_associative : AA.Associative (α := ℕ) (· + ·)
+/-- Exchanging the operands of an addition does not change the result. -/
+theorem add_comm {n m : ℕ} : n + m ≃ m + n := by
+  apply ind_on (motive := λ n => n + m ≃ m + n) n
+  case zero =>
+    show 0 + m ≃ m + 0
+    calc
+      0 + m ≃ _ := Addition.zero_add
+      m     ≃ _ := Rel.symm add_zero
+      m + 0 ≃ _ := Rel.refl
+  case step =>
+    intro n (ih : n + m ≃ m + n)
+    show step n + m ≃ m + step n
+    calc
+      step n + m   ≃ _ := Addition.step_add
+      step (n + m) ≃ _ := AA.subst₁ ih
+      step (m + n) ≃ _ := Rel.symm add_step
+      m + step n   ≃ _ := Rel.refl
 
-  /--
-  The same quantity can be removed (cancelled) from both sides of an equality
-  of sums.
-  -/
-  add_cancellative : AA.Cancellative (α := ℕ) (· + ·) AA.tc (· ≃ ·) (· ≃ ·)
+instance add_commutative : AA.Commutative (α := ℕ) (· + ·) where
+  comm := add_comm
 
-  /--
-  Both operands in a sum of natural numbers must be zero if the result is zero.
-  -/
-  zero_sum_split {n m : ℕ} : n + m ≃ 0 → n ≃ 0 ∧ m ≃ 0
+/--
+Addition preserves equivalence of natural numbers; two equivalent natural
+numbers are still equivalent after the same quantity is added to both (on the
+right).
+-/
+theorem subst_add {n₁ n₂ m : ℕ} : n₁ ≃ n₂ → n₁ + m ≃ n₂ + m := by
+  apply ind_on (motive := λ x => ∀ y, x ≃ y → x + m ≃ y + m) n₁
+  case zero =>
+    intro n₂
+    show 0 ≃ n₂ → 0 + m ≃ n₂ + m
+    apply cases_on (motive := λ y => 0 ≃ y → 0 + m ≃ y + m)
+    case zero =>
+      intro (_ : 0 ≃ (0 : ℕ))
+      show 0 + m ≃ 0 + m
+      exact Rel.refl
+    case step =>
+      intro n₂ (_ : 0 ≃ step n₂)
+      show 0 + m ≃ step n₂ + m
+      apply False.elim
+      show False
+      exact Axioms.step_neq_zero (Rel.symm ‹0 ≃ step n₂›)
+  case step =>
+    intro n₁ (ih : ∀ y, n₁ ≃ y → n₁ + m ≃ y + m) n₂
+    show step n₁ ≃ n₂ → step n₁ + m ≃ n₂ + m
+    apply cases_on (motive := λ y => step n₁ ≃ y → step n₁ + m ≃ y + m)
+    case zero =>
+      intro (_ : step n₁ ≃ 0)
+      show step n₁ + m ≃ 0 + m
+      apply False.elim
+      show False
+      exact Axioms.step_neq_zero ‹step n₁ ≃ 0›
+    case step =>
+      intro n₂ (_ : step n₁ ≃ step n₂)
+      show step n₁ + m ≃ step n₂ + m
+      have : n₁ ≃ n₂ := AA.inject ‹step n₁ ≃ step n₂›
+      calc
+        step n₁ + m   ≃ _ := Addition.step_add
+        step (n₁ + m) ≃ _ := AA.subst₁ (ih _ ‹n₁ ≃ n₂›)
+        step (n₂ + m) ≃ _ := Rel.symm Addition.step_add
+        step n₂ + m   ≃ _ := Rel.refl
 
-attribute [instance] Addition.Derived.add_associative
-attribute [instance] Addition.Derived.add_cancellative
-attribute [instance] Addition.Derived.add_commutative
-attribute [instance] Addition.Derived.add_identity
-attribute [instance] Addition.Derived.add_semicompatible_step
-attribute [instance] Addition.Derived.add_substitutive
+def add_substL
+    : AA.SubstitutiveOn Hand.L (α := ℕ) (· + ·) AA.tc (· ≃ ·) (· ≃ ·) where
+  subst₂ := λ (_ : True) => subst_add
 
-namespace Addition
-export Addition.Base (addOp step_add zero_add)
-export Addition.Derived (
-  add_associative add_cancellative add_commutative add_one_step add_step
-  add_substitutive add_zero zero_sum_split
-)
-end Addition
+instance add_substitutive
+    : AA.Substitutive₂ (α := ℕ) (· + ·) AA.tc (· ≃ ·) (· ≃ ·) where
+  substitutiveL := add_substL
+  substitutiveR := AA.substR_from_substL_swap (rS := (· ≃ ·)) add_substL
+
+/-- Adding one is the same as incrementing. -/
+theorem add_one_step {n : ℕ} : n + 1 ≃ step n := by
+  calc
+    n + 1        ≃ _ := AA.substR Literals.literal_step
+    n + step 0   ≃ _ := add_step
+    step (n + 0) ≃ _ := AA.subst₁ add_zero
+    step n       ≃ _ := Rel.refl
+
+/--
+The grouping of the terms in a sum doesn't matter.
+
+**Intuition**: the `step_add` and `add_step` properties allow `step`s to be
+moved arbitrarily between terms. Given any particular grouping of a sum, all of
+the `step`s can be moved over to the first term, always producing the same
+result.
+-/
+instance add_associative : AA.Associative (α := ℕ) (· + ·) := by
+  constructor
+  intro n m k
+  show (n + m) + k ≃ n + (m + k)
+  apply ind_on (motive := λ n => (n + m) + k ≃ n + (m + k)) n
+  case zero =>
+    show (0 + m) + k ≃ 0 + (m + k)
+    calc
+      (0 + m) + k ≃ _ := AA.substL Addition.zero_add
+      m + k       ≃ _ := Rel.symm Addition.zero_add
+      0 + (m + k) ≃ _ := Rel.refl
+  case step =>
+    intro n (ih : (n + m) + k ≃ n + (m + k))
+    show (step n + m) + k ≃ step n + (m + k)
+    calc
+      (step n + m) + k   ≃ _ := AA.substL Addition.step_add
+      step (n + m) + k   ≃ _ := Addition.step_add
+      step ((n + m) + k) ≃ _ := AA.subst₁ ih
+      step (n + (m + k)) ≃ _ := Rel.symm Addition.step_add
+      step n + (m + k)   ≃ _ := Rel.refl
+
+/--
+The right-hand sides of two equal sums are equal if their left-hand sides are.
+
+**Proof intuition**: the left-hand sides can be removed one `step` at a time by
+applying `step_injective` and finally `zero_add`, leaving the desired result.
+-/
+theorem cancel_add {n m k : ℕ} : n + m ≃ n + k → m ≃ k := by
+  apply ind_on (motive := λ n => n + m ≃ n + k → m ≃ k) n
+  case zero =>
+    intro (_ : 0 + m ≃ 0 + k)
+    show m ≃ k
+    calc
+      m     ≃ _ := Rel.symm Addition.zero_add
+      0 + m ≃ _ := ‹0 + m ≃ 0 + k›
+      0 + k ≃ _ := Addition.zero_add
+      k     ≃ _ := Rel.refl
+  case step =>
+    intro n (ih : n + m ≃ n + k → m ≃ k) (_ : step n + m ≃ step n + k)
+    show m ≃ k
+    apply ih
+    show n + m ≃ n + k
+    apply AA.inject (β := ℕ) (f := step) (rβ := (· ≃ ·))
+    show step (n + m) ≃ step (n + k)
+    calc
+      step (n + m) ≃ _ := Rel.symm Addition.step_add
+      step n + m   ≃ _ := ‹step n + m ≃ step n + k›
+      step n + k   ≃ _ := Addition.step_add
+      step (n + k) ≃ _ := Rel.refl
+
+def add_cancelL
+    : AA.CancellativeOn Hand.L (α := ℕ) (· + ·) AA.tc (· ≃ ·) (· ≃ ·) := {
+  cancel := λ (_ : True) => cancel_add
+}
+
+instance add_cancellative
+    : AA.Cancellative (α := ℕ) (· + ·) AA.tc (· ≃ ·) (· ≃ ·) := {
+  cancellativeL := add_cancelL
+  cancellativeR := AA.cancelR_from_cancelL add_cancelL
+}
+
+/--
+Both operands in a sum of natural numbers must be zero if the result is zero.
+-/
+theorem zero_sum_split {n m : ℕ} : n + m ≃ 0 → n ≃ 0 ∧ m ≃ 0 := by
+  apply cases_on (motive := λ n => n + m ≃ 0 → n ≃ 0 ∧ m ≃ 0) n
+  case zero =>
+    intro (_ : 0 + m ≃ 0)
+    show 0 ≃ 0 ∧ m ≃ 0
+    have : m ≃ 0 := Rel.trans (Rel.symm Addition.zero_add) ‹0 + m ≃ 0›
+    exact And.intro Rel.refl ‹m ≃ 0›
+  case step =>
+    intro n (_ : step n + m ≃ 0)
+    show step n ≃ 0 ∧ m ≃ 0
+    apply False.elim
+    show False
+    have : step (n + m) ≃ 0 :=
+      Rel.trans (Rel.symm Addition.step_add) ‹step n + m ≃ 0›
+    exact Axioms.step_neq_zero ‹step (n + m) ≃ 0›
 
 end Lean4Axiomatic.Natural
