git/cruhland/lean4-axiomatic/Lean4Axiomatic/Natural.lean
@@ -21,7 +21,7 @@ required to construct an instance.
 class Natural (ℕ : Type) where
   toCore : Core ℕ
   toAxioms : Axioms ℕ
-  toAddition : Addition.Derived ℕ
+  toAddition : Addition ℕ
   toSign : Sign ℕ
   toOrder : Order.Derived ℕ
   toMultiplication : Multiplication.Derived ℕ
@@ -36,14 +36,7 @@ attribute [instance] toMultiplication
 attribute [instance] toOrder
 attribute [instance] toSign
 
-export Addition (
-  add_associative add_cancellative add_commutative add_one_step addOp add_step
-  add_substitutive add_zero step_add zero_add zero_sum_split
-)
-export Core (step_substitutive)
-export Equality (eqvOp?)
 export Exponentiation (powOp pow_step pow_zero)
-export Literals (literal literal_step literal_zero)
 export Multiplication (
   mul_associative mul_cancellative mul_commutative mul_distributive mulOp
   mul_positive mul_split_zero mul_step mul_substitutive_eq mul_substitutive_lt
@@ -54,6 +47,5 @@ export Order (
   lt_defn lt_defn_add ltOp lt_split lt_step lt_step_le lt_zero lt_zero_pos
   trichotomy
 )
-export Sign (positive_add positive_step)
 
 end Lean4Axiomatic.Natural
