git/cruhland/lean4-axiomatic/Lean4Axiomatic/Natural/Impl/Derived.lean
@@ -1,3 +1,2 @@
-import Lean4Axiomatic.Natural.Impl.Derived.Addition
 import Lean4Axiomatic.Natural.Impl.Derived.Multiplication
 import Lean4Axiomatic.Natural.Impl.Derived.Order
